intermediate/Veritas.Intermediate.Store.fst
@@ -5,25 +5,37 @@ let update_slot #vcfg (st:vstore_raw vcfg) (s:slot_id vcfg) (e:vstore_entry vcfg
   : vstore_raw _
   = Seq.upd st s (Some e)
 
-let points_to_unchanged_slot #vcfg (st1 st2: vstore_raw vcfg) (s: slot_id vcfg) = 
+let points_to_unchanged_slot #vcfg (st1 st2: vstore_raw vcfg) (s: slot_id vcfg) =
   inuse_slot st1 s = inuse_slot st2 s /\
   (inuse_slot st1 s ==> points_to_info st1 s Left = points_to_info st2 s Left /\
                        points_to_info st1 s Right = points_to_info st2 s Right)
-                       
-let points_to_unchanged #vcfg (st1 st2: vstore_raw vcfg) = 
-  forall (s: slot_id vcfg). {:pattern points_to_unchanged_slot st1 st2 s} 
+
+let points_to_unchanged #vcfg (st1 st2: vstore_raw vcfg) =
+  forall (s: slot_id vcfg). {:pattern points_to_unchanged_slot st1 st2 s}
                        points_to_unchanged_slot st1 st2 s
 
+/// Two stores have the same slot or the slot is empty for a given slot s
+///
+let add_method_unchanged_slot #vcfg (st1 st2: vstore_raw vcfg) (s: slot_id vcfg) =
+  inuse_slot st1 s = inuse_slot st2 s /\
+  (inuse_slot st1 s ==> add_method_of st1 s = add_method_of st2 s)
+
+/// Two stores have the same empty slots and the same add methods for non-empty slots
+///
+let add_method_unchanged #vcfg (st1 st2: vstore_raw vcfg) =
+  forall (s: slot_id vcfg). {:pattern add_method_unchanged_slot st1 st2 s} add_method_unchanged_slot st1 st2 s
+
 let lemma_points_to_unchanged_implies_points_to_inuse #vcfg (st1 st2: vstore_raw vcfg)
-  : Lemma (requires (points_to_unchanged st1 st2 /\ points_to_inuse st1))
+  : Lemma (requires (points_to_unchanged st1 st2 /\ points_to_inuse st1 /\ add_method_unchanged st1 st2))
           (ensures (points_to_inuse st2))
-          [SMTPat (points_to_unchanged st1 st2)] = 
+          [SMTPat (points_to_unchanged st1 st2)] =
   let aux (s1 s2: slot_id vcfg):
     Lemma (ensures (points_to_inuse_local st2 s1 s2))
-          [SMTPat (points_to_inuse_local st2 s1 s2)] = 
+          [SMTPat (points_to_inuse_local st2 s1 s2)] =
     assert(points_to_unchanged_slot st1 st2 s1);
     assert(points_to_unchanged_slot st1 st2 s2);
     assert(points_to_inuse_local st1 s1 s2);
+    assert(add_method_unchanged_slot st1 st2 s2);
     ()
   in
   ()
@@ -31,59 +43,59 @@ let lemma_points_to_unchanged_implies_points_to_inuse #vcfg (st1 st2: vstore_raw
 let slot_dir vcfg = (slot_id vcfg) & bin_tree_dir
 
 let pointed_dir #vcfg (st: vstore_raw vcfg) (s1: slot_id vcfg) (s2: slot_id _{points_to st s1 s2}):
-  (d:bin_tree_dir{points_to_dir st s1 d s2}) = 
+  (d:bin_tree_dir{points_to_dir st s1 d s2}) =
   if points_to_dir st s1 Left s2 then Left
   else Right
 
 /// Computational version of pointed_to_inv_local
 ///
-let rec pointed_to_inv_local_find_aux #vcfg (st: vstore_raw vcfg) 
+let rec pointed_to_inv_local_find_aux #vcfg (st: vstore_raw vcfg)
                                         (s: slot_id vcfg{pointed_to_inv_local st s /\
                                                          inuse_slot st s /\
                                                          stored_key st s <> Root /\
                                                          add_method_of st s = Spec.MAdd})
-                                        (sl: nat{sl <= store_size vcfg})     // slot limit 
+                                        (sl: nat{sl <= store_size vcfg})     // slot limit
   : (r:option (slot_dir vcfg){r = None /\
-                              (forall (s1:slot_id vcfg{s1 < sl}). forall (d:bin_tree_dir). 
+                              (forall (s1:slot_id vcfg{s1 < sl}). forall (d:bin_tree_dir).
                                 empty_slot st s1 \/
-                                points_to_none st s1 d \/ 
+                                points_to_none st s1 d \/
                                 pointed_slot st s1 d <> s) \/
                               Some? r /\ (let (s1,d) = Some?.v r in
                                           inuse_slot st s1 /\
                                           points_to_some_slot st s1 d /\
                                           pointed_slot st s1 d = s)})
-  = 
+  =
   if sl = 0 then None
   else
-    let sl' = sl - 1 in 
+    let sl' = sl - 1 in
     let r' = pointed_to_inv_local_find_aux st s sl' in
     if Some? r' then
       Some (Some?.v r')
     else
       if inuse_slot st sl' && points_to st sl' s then
         let d = pointed_dir st sl' s in
-        Some (sl', d)     
+        Some (sl', d)
       else
         let aux(d:bin_tree_dir)
           : Lemma (forall (s1:slot_id vcfg{s1 < sl}).
-                     empty_slot st s1 \/ points_to_none st s1 d \/ pointed_slot st s1 d <> s) 
-          =           
+                     empty_slot st s1 \/ points_to_none st s1 d \/ pointed_slot st s1 d <> s)
+          =
           let aux2 (s1:slot_id vcfg{s1 < sl})
             : Lemma (empty_slot st s1 \/ points_to_none st s1 d \/ pointed_slot st s1 d <> s)
-            = 
+            =
             if s1 = sl' then ()
             else
-              () 
-            
-          in            
+              ()
+
+          in
           forall_intro aux2
         in
         forall_intro aux;
-        None     
+        None
 
 /// For a slot s added with Merkle, use the invariant to find another slot pointing to s
-/// 
-let pointed_to_inv_local_find #vcfg (st: vstore_raw vcfg) 
+///
+let pointed_to_inv_local_find #vcfg (st: vstore_raw vcfg)
                                     (s: slot_id vcfg{pointed_to_inv_local st s /\
                                                          inuse_slot st s /\
                                                          stored_key st s <> Root /\
@@ -92,22 +104,22 @@ let pointed_to_inv_local_find #vcfg (st: vstore_raw vcfg)
                          inuse_slot st s1 /\
                          points_to_some_slot st s1 d /\
                          pointed_slot st s1 d = s})
-  = 
+  =
   let r = pointed_to_inv_local_find_aux st s (store_size vcfg) in
   if r = None then (
     assert(pointed_to_inv_local st s);
     let aux (d:bin_tree_dir)
       : Lemma (ensures (forall (s':inuse_slot_id st). ~ (points_to_some_slot st s' d /\ pointed_slot st s' d = s)))
-      = 
+      =
       let aux2 (s':inuse_slot_id st):
         Lemma (ensures (~ (points_to_some_slot st s' d /\ pointed_slot st s' d = s)))
-        = 
+        =
         assert(empty_slot st s' \/
-               points_to_none st s' d \/ 
+               points_to_none st s' d \/
                pointed_slot st s' d <> s);
         ()
       in
-      forall_intro aux2      
+      forall_intro aux2
     in
     forall_intro aux;
     // assert (forall (s':inuse_slot_id st) (d:bin_tree_dir). ~ (points_to_some_slot st s' d /\ pointed_slot st s' d = s));
@@ -117,48 +129,37 @@ let pointed_to_inv_local_find #vcfg (st: vstore_raw vcfg)
   else Some?.v r
 
 /// Two stores have the the same key or the slot is empty for a given slot s
-/// 
-let keys_unchanged_slot #vcfg (st1 st2: vstore_raw vcfg) (s: slot_id vcfg) = 
+///
+let keys_unchanged_slot #vcfg (st1 st2: vstore_raw vcfg) (s: slot_id vcfg) =
   inuse_slot st1 s = inuse_slot st2 s /\
   (inuse_slot st1 s ==> stored_key st1 s = stored_key st2 s)
 
 /// Two stores have the same empty slots and the same keys in non-empty slots
-/// 
-let keys_unchanged #vcfg (st1 st2: vstore_raw vcfg) = 
-  forall (s: slot_id vcfg). {:pattern keys_unchanged_slot st1 st2 s} 
+///
+let keys_unchanged #vcfg (st1 st2: vstore_raw vcfg) =
+  forall (s: slot_id vcfg). {:pattern keys_unchanged_slot st1 st2 s}
                        keys_unchanged_slot st1 st2 s
-
-/// Two stores have the same slot or the slot is empty for a given slot s
-/// 
-let add_method_unchanged_slot #vcfg (st1 st2: vstore_raw vcfg) (s: slot_id vcfg) =
-  inuse_slot st1 s = inuse_slot st2 s /\
-  (inuse_slot st1 s ==> add_method_of st1 s = add_method_of st2 s)
-
-/// Two stores have the same empty slots and the same add methods for non-empty slots
-/// 
-let add_method_unchanged #vcfg (st1 st2: vstore_raw vcfg) = 
-  forall (s: slot_id vcfg). {:pattern add_method_unchanged_slot st1 st2 s} add_method_unchanged_slot st1 st2 s
 
 let lemma_points_to_unchanged_implies_pointed_to_inv_local #vcfg (st1 st2: vstore_raw vcfg) (s:slot_id vcfg)
   : Lemma (requires (points_to_unchanged st1 st2 /\ keys_unchanged st1 st2 /\ add_method_unchanged st1 st2 /\ pointed_to_inv_local st1 s))
-          (ensures (pointed_to_inv_local st2 s)) = 
+          (ensures (pointed_to_inv_local st2 s)) =
   if empty_slot st1 s then
-    assert(points_to_unchanged_slot st1 st2 s)  
+    assert(points_to_unchanged_slot st1 st2 s)
   else if stored_key st1 s = Root then
     assert(keys_unchanged_slot st1 st2 s)
   else if add_method_of st1 s <> Spec.MAdd then
     assert(add_method_unchanged_slot st1 st2 s)
-  else (    
+  else (
     let (s',d) = pointed_to_inv_local_find st1 s in
     assert(points_to_unchanged_slot st1 st2 s');
-  
+
     let aux (d1: bin_tree_dir):Type0 = points_to_dir st2 s' d1 s in
     exists_intro aux d;
     assert(exists d1. points_to_dir st2 s' d1 s);
 
     let aux (s1: inuse_slot_id st2) = exists d1. points_to_dir st2 s1 d1 s in
     exists_intro aux s';
-    
+
     // assert (exists (s1: inuse_slot_id st2). exists (d1: bin_tree_dir). points_to_dir st2 s1 d1 s);
 
     ()
@@ -167,7 +168,7 @@ let lemma_points_to_unchanged_implies_pointed_to_inv_local #vcfg (st1 st2: vstor
 let lemma_points_to_unchanged_implies_pointed_to_inv #vcfg (st1 st2: vstore_raw vcfg)
   : Lemma (requires (points_to_unchanged st1 st2 /\ keys_unchanged st1 st2 /\ add_method_unchanged st1 st2 /\ pointed_to_inv st1))
           (ensures (pointed_to_inv st2))
-          [SMTPat (points_to_unchanged st1 st2)] = 
+          [SMTPat (points_to_unchanged st1 st2)] =
   let aux (s: slot_id vcfg)
     : Lemma (ensures (pointed_to_inv_local st2 s))
             [SMTPat (pointed_to_inv_local st2 s)]
@@ -181,8 +182,8 @@ let lemma_points_to_unchanged_implies_points_to_uniq #vcfg (st1 st2: vstore_raw 
           [SMTPat (points_to_unchanged st1 st2)] =
   let aux (s1 s2 s: slot_id vcfg)
     : Lemma (ensures (points_to_uniq_local st2 s1 s2 s))
-            [SMTPat (points_to_uniq_local st2 s1 s2 s)] = 
-    assert(points_to_uniq_local st1 s1 s2 s);            
+            [SMTPat (points_to_uniq_local st2 s1 s2 s)] =
+    assert(points_to_uniq_local st1 s1 s2 s);
     assert(points_to_unchanged_slot st1 st2 s1);
     assert(points_to_unchanged_slot st1 st2 s2);
     ()
@@ -190,21 +191,21 @@ let lemma_points_to_unchanged_implies_points_to_uniq #vcfg (st1 st2: vstore_raw 
   ()
 
 let update_value_raw #vcfg (st:vstore vcfg) (s:inuse_slot_id st) (v:value_type_of (stored_key st s))
-  : vstore_raw vcfg = 
+  : vstore_raw vcfg =
   let VStoreE k v' am lp rp = get_inuse_slot st s in
   let e' = VStoreE k v am lp rp in
   update_slot st s e'
 
-let lemma_update_value_identical_except 
+let lemma_update_value_identical_except
   #vcfg (st:vstore vcfg) (s:inuse_slot_id st) (v:value_type_of (stored_key st s))
-  : Lemma (ensures (let st' = update_value_raw st s v in 
+  : Lemma (ensures (let st' = update_value_raw st s v in
                     identical_except st st' s))
-          [SMTPat (update_value_raw st s v)] = 
-  let st' = update_value_raw st s v in                    
+          [SMTPat (update_value_raw st s v)] =
+  let st' = update_value_raw st s v in
   let aux (s': slot_id vcfg)
     : Lemma (ensures (s' <> s ==> get_slot st s' = get_slot st' s'))
             [SMTPat (get_slot st s' = get_slot st' s')]
-    = 
+    =
     ()
   in
   ()
@@ -213,11 +214,11 @@ let lemma_update_value_keys_unchanged
   #vcfg (st:vstore vcfg) (s:inuse_slot_id st) (v:value_type_of (stored_key st s))
   : Lemma (ensures (let st' = update_value_raw st s v in
                     keys_unchanged st st'))
-          [SMTPat (update_value_raw st s v)] = 
-  let st' = update_value_raw st s v in                    
+          [SMTPat (update_value_raw st s v)] =
+  let st' = update_value_raw st s v in
   let aux(s2: slot_id vcfg)
     : Lemma (ensures (keys_unchanged_slot st st' s2))
-            [SMTPat (keys_unchanged_slot st st' s2)] = 
+            [SMTPat (keys_unchanged_slot st st' s2)] =
     ()
   in
   ()
@@ -226,11 +227,11 @@ let lemma_update_value_add_method_unchaged
   #vcfg (st:vstore vcfg) (s:inuse_slot_id st) (v:value_type_of (stored_key st s))
   : Lemma (ensures (let st' = update_value_raw st s v in
                     add_method_unchanged st st'))
-          [SMTPat (update_value_raw st s v)] = 
+          [SMTPat (update_value_raw st s v)] =
   let st' = update_value_raw st s v in
   let aux (s2: slot_id vcfg)
     : Lemma (ensures (add_method_unchanged_slot st st' s2))
-            [SMTPat (add_method_unchanged_slot st st' s2)] = 
+            [SMTPat (add_method_unchanged_slot st st' s2)] =
     ()
   in
   ()
@@ -239,16 +240,16 @@ let lemma_update_value_points_to_unchanged
   #vcfg (st:vstore vcfg) (s:inuse_slot_id st) (v: value_type_of (stored_key st s))
   : Lemma (ensures (let st' = update_value_raw st s v in
                     points_to_unchanged st st'))
-          [SMTPat (update_value_raw st s v)] = 
+          [SMTPat (update_value_raw st s v)] =
   let st' = update_value_raw st s v in
   let aux (s2: slot_id vcfg)
     : Lemma (ensures (points_to_unchanged_slot st st' s2))
-            [SMTPat (points_to_unchanged_slot st st' s2)] = 
+            [SMTPat (points_to_unchanged_slot st st' s2)] =
     ()
   in
   ()
 
-let update_value 
+let update_value
   (#vcfg:_)
   (st:vstore vcfg)
   (s:inuse_slot_id st)
@@ -258,11 +259,11 @@ let update_value
                           v = stored_value st' s /\
                           (let VStoreE k1 _ am1 ld1 rd1 = get_inuse_slot st s in
                            let VStoreE k2 _ am2 ld2 rd2 = get_inuse_slot st' s in
-                           k1 = k2 /\ am1 = am2 /\ ld1 = ld2 /\ rd1 = rd2)}) = 
-  update_value_raw st s v 
+                           k1 = k2 /\ am1 = am2 /\ ld1 = ld2 /\ rd1 = rd2)}) =
+  update_value_raw st s v
 
 /// The "raw" version of madd_to_store on which we prove properties
-/// 
+///
 let madd_to_store_raw
   (#vcfg: verifier_config)
   (st: vstore vcfg)
@@ -270,7 +271,7 @@ let madd_to_store_raw
   (k:key) (v:value_type_of k)
   (s':merkle_slot_id st)
   (d:bin_tree_dir {points_to_none st s' d})
-  : Tot (vstore_raw vcfg) = 
+  : Tot (vstore_raw vcfg) =
   let e = VStoreE k v Spec.MAdd None None in
   let st = update_slot st s e in
   let VStoreE k' v' am' l' r' = get_inuse_slot st s' in
@@ -278,8 +279,8 @@ let madd_to_store_raw
 
   if d = Left then
     update_slot st s' (VStoreE k' v' am' (Some s) r')
-  else 
-    update_slot st s' (VStoreE k' v' am' l' (Some s))  
+  else
+    update_slot st s' (VStoreE k' v' am' l' (Some s))
 
 let lemma_madd_to_store_identical_except
   (#vcfg: verifier_config)
@@ -290,8 +291,8 @@ let lemma_madd_to_store_identical_except
   (d:bin_tree_dir {points_to_none st s' d})
   : Lemma (ensures (let st' = madd_to_store_raw st s k v s' d in
                     identical_except2 st st' s s'))
-          [SMTPat (madd_to_store_raw st s k v s' d)] = 
-  let st' = madd_to_store_raw st s k v s' d in          
+          [SMTPat (madd_to_store_raw st s k v s' d)] =
+  let st' = madd_to_store_raw st s k v s' d in
   let aux (s2: slot_id _)
     : Lemma (ensures (s2 <> s ==> s2 <> s' ==> get_slot st s2 = get_slot st' s2))
             [SMTPat (get_slot st s2 = get_slot st' s2)] =
@@ -313,11 +314,11 @@ let lemma_madd_to_store_points_to_inuse
   (d:bin_tree_dir {points_to_none st s' d})
   : Lemma (ensures (let st' = madd_to_store_raw st s k v s' d in
                     points_to_inuse st'))
-          [SMTPat (madd_to_store_raw st s k v s' d)] = 
+          [SMTPat (madd_to_store_raw st s k v s' d)] =
   let st' = madd_to_store_raw st s k v s' d in
   let aux (s1 s2: slot_id _)
     : Lemma (ensures (points_to_inuse_local st' s1 s2))
-            [SMTPat (points_to_inuse_local st' s1 s2)] = 
+            [SMTPat (points_to_inuse_local st' s1 s2)] =
     assert(points_to_inuse_local st s1 s2);
     ()
   in
@@ -334,12 +335,12 @@ let lemma_madd_to_store_points_to_uniq
   (d:bin_tree_dir {points_to_none st s' d})
   : Lemma (ensures (let st' = madd_to_store_raw st s k v s' d in
                     points_to_uniq st'))
-          [SMTPat (madd_to_store_raw st s k v s' d)] = 
+          [SMTPat (madd_to_store_raw st s k v s' d)] =
   let st' = madd_to_store_raw st s k v s' d in
   let aux (s1 s2 s3: _):
     Lemma (ensures (points_to_uniq_local st' s1 s2 s3))
-          [SMTPat (points_to_uniq_local st' s1 s2 s3)] = 
-    assert(points_to_uniq_local st s1 s2 s3);          
+          [SMTPat (points_to_uniq_local st' s1 s2 s3)] =
+    assert(points_to_uniq_local st s1 s2 s3);
     if points_to_uniq_local st' s1 s2 s3 then ()
     else (
       assert(points_to st' s1 s3 && points_to st' s2 s3);
@@ -397,14 +398,14 @@ let exists_intro_helper #vcfg
                     exists (s2:inuse_slot_id st). exists (d2:bin_tree_dir).
                       points_to_some_slot st s2 d2 /\
                       pointed_slot st s2 d2 = s))
-          [SMTPat (pointed_slot st s' d)] = 
-  let s = pointed_slot st s' d in          
+          [SMTPat (pointed_slot st s' d)] =
+  let s = pointed_slot st s' d in
   let aux(d1: bin_tree_dir): Type0 = points_to_dir st s' d1 s in
   exists_intro aux d;
   let aux(s1:inuse_slot_id st) = exists d1. points_to_dir st s1 d1 s in
   exists_intro aux s'
 
-let lemma_madd_to_store_pointed_to_inverse_local 
+let lemma_madd_to_store_pointed_to_inverse_local
   (#vcfg: verifier_config)
   (st: vstore vcfg)
   (s:empty_slot_id st)
@@ -413,9 +414,9 @@ let lemma_madd_to_store_pointed_to_inverse_local
   (d:bin_tree_dir {points_to_none st s' d})
   (s2: slot_id vcfg)
   : Lemma (ensures (let st' = madd_to_store_raw st s k v s' d in
-                    pointed_to_inv_local st' s2)) 
-          [SMTPat (pointed_to_inv_local (madd_to_store_raw st s k v s' d) s2)]                    
-  = let st' = madd_to_store_raw st s k v s' d in  
+                    pointed_to_inv_local st' s2))
+          [SMTPat (pointed_to_inv_local (madd_to_store_raw st s k v s' d) s2)]
+  = let st' = madd_to_store_raw st s k v s' d in
     if empty_slot st' s2 || stored_key st' s2 = Root || add_method_of st' s2 <> Spec.MAdd then ()
     else (
       if s2 = s then (
@@ -435,7 +436,7 @@ let lemma_madd_to_store_pointed_to_inverse_local
         assert(s2' <> s' \/ d2 <> d);
 
         // assert(points_to_some_slot st' s2' d2);
-        assert(pointed_slot st' s2' d2 = s2);        
+        assert(pointed_slot st' s2' d2 = s2);
         ()
       )
     )
@@ -450,7 +451,7 @@ let lemma_madd_to_store_pointed_to_inverse
   : Lemma (ensures (let st' = madd_to_store_raw st s k v s' d in
                     pointed_to_inv st'))
           [SMTPat (madd_to_store_raw st s k v s' d)] = ()
-       
+
 let madd_to_store
   (#vcfg: verifier_config)
   (st:vstore vcfg)
@@ -471,11 +472,11 @@ let madd_to_store
 
                          // slot s contains (k, v, MAdd) and points to nothing
                          inuse_slot st' s /\
-                         get_inuse_slot st' s = VStoreE k v Spec.MAdd None None                         
+                         get_inuse_slot st' s = VStoreE k v Spec.MAdd None None
                          })
   = madd_to_store_raw st s k v s' d
 
-let madd_to_store_split_raw 
+let madd_to_store_split_raw
   (#vcfg: verifier_config)
   (st:vstore vcfg)
   (s:empty_slot_id st)
@@ -483,11 +484,11 @@ let madd_to_store_split_raw
   (s':merkle_slot_id st)
   (d:bin_tree_dir {points_to_some_slot st s' d})
   (d2:bin_tree_dir)
-  : vstore_raw  vcfg = 
+  : vstore_raw  vcfg =
 
   let s2 = pointed_slot st s' d in
-  let VStoreE k' v' am' l' r' = get_inuse_slot st s' in  
-  let e = (if d2 = Left then 
+  let VStoreE k' v' am' l' r' = get_inuse_slot st s' in
+  let e = (if d2 = Left then
              VStoreE k v Spec.MAdd (Some s2) None
            else
              VStoreE k v Spec.MAdd None (Some s2))
@@ -509,11 +510,11 @@ let lemma_madd_to_store_split_identical_except
   (d2:bin_tree_dir)
   : Lemma (ensures (let st' = madd_to_store_split_raw st s k v s' d d2 in
                     identical_except2 st st' s s'))
-          [SMTPat (madd_to_store_split_raw st s k v s' d d2)] = 
+          [SMTPat (madd_to_store_split_raw st s k v s' d d2)] =
   let st' = madd_to_store_split_raw st s k v s' d d2 in
   let aux (s2: slot_id _)
     : Lemma (ensures (s2 <> s ==> s2 <> s' ==> get_slot st s2 = get_slot st' s2))
-            [SMTPat (get_slot st s2 = get_slot st' s2)] = 
+            [SMTPat (get_slot st s2 = get_slot st' s2)] =
     if s2 = s then ()
     else if s2 = s' then ()
     else ()
@@ -529,12 +530,12 @@ let lemma_madd_to_store_split_points_to_inuse
   (d2:bin_tree_dir)
   : Lemma (ensures (let st' = madd_to_store_split_raw st s k v s' d d2 in
                     points_to_inuse st'))
-          [SMTPat (madd_to_store_split_raw st s k v s' d d2)] = 
+          [SMTPat (madd_to_store_split_raw st s k v s' d d2)] =
   let st' = madd_to_store_split_raw st s k v s' d d2 in
   let aux (s1 s2: slot_id _)
     : Lemma (ensures (points_to_inuse_local st' s1 s2))
             [SMTPat (points_to_inuse_local st' s1 s2)] =
-    assert(points_to_inuse_local st s1 s2); 
+    assert(points_to_inuse_local st s1 s2);
     if not (points_to st' s1 s2) then ()
     else (
       let d12 = pointed_dir st' s1 s2 in
@@ -555,7 +556,7 @@ let lemma_madd_to_store_split_points_to_inuse
   in
   ()
 
-let madd_to_store_split 
+let madd_to_store_split
   (#vcfg: verifier_config)
   (st:vstore vcfg)
   (s:empty_slot_id st)
@@ -563,14 +564,14 @@ let madd_to_store_split
   (s':merkle_slot_id st)
   (d:bin_tree_dir {points_to_some_slot st s' d})
   (d2:bin_tree_dir)
-  : Tot (st': vstore vcfg{let od = other_dir d in        
+  : Tot (st': vstore vcfg{let od = other_dir d in
                           let s2 = pointed_slot st s' d in
                           let od2 = other_dir d2 in
-                          
+
                           // st and st' identical except at s, s'
                           identical_except2 st st' s s' /\
 
-                          // nothing changes in slot s', except it now points to s in direction d 
+                          // nothing changes in slot s', except it now points to s in direction d
                           inuse_slot st' s' /\
                           stored_key st' s' = stored_key st s' /\
                           stored_value st' s' = stored_value st s' /\
@@ -593,31 +594,31 @@ let madd_to_store_root
   : Tot (st':vstore vcfg{// st and st' identical except at s, s'
                          identical_except st st' s /\
 
-                         // slot s contains (Root, v, MAdd) and points to none 
+                         // slot s contains (Root, v, MAdd) and points to none
                          inuse_slot st' s /\
-                         get_inuse_slot st' s = VStoreE Root v Spec.MAdd None None})                        
+                         get_inuse_slot st' s = VStoreE Root v Spec.MAdd None None})
   = admit()
 
-let badd_to_store 
+let badd_to_store
       (#vcfg:verifier_config)
-      (st:vstore vcfg) 
+      (st:vstore vcfg)
       (s:empty_slot_id st)
-      (k:key) 
-      (v:value_type_of k) 
+      (k:key)
+      (v:value_type_of k)
   : Tot (st':vstore vcfg {// st and st' identical except for s
                           identical_except st st' s /\
                           inuse_slot st' s /\
                           get_inuse_slot st' s = VStoreE k v Spec.BAdd None None})
   = admit()
 
-let mevict_from_store 
+let mevict_from_store
   (#vcfg: verifier_config)
   (st:vstore vcfg)
-  (s:inuse_slot_id st{points_to_none st s Left /\ points_to_none st s Right})  
+  (s:inuse_slot_id st{points_to_none st s Left /\ points_to_none st s Right})
   (s':inuse_slot_id st)
   (d:bin_tree_dir{points_to_dir st s' d s})
   : Tot (st':vstore vcfg {let od = other_dir d in
-                          
+
                           // st and st' identical except at s, s'
                           identical_except2 st st' s s' /\
 
@@ -638,15 +639,15 @@ let bevict_from_store
   (#vcfg: verifier_config)
   (st:vstore vcfg)
   (s:inuse_slot_id st{points_to_none st s Left /\ points_to_none st s Right})
-  : Tot (st':vstore vcfg {// st and st' are identical except at slot s 
+  : Tot (st':vstore vcfg {// st and st' are identical except at slot s
                           identical_except st st' s /\
 
                           // slot s is empty after the update
                           empty_slot st' s})
   = admit()
 
-let pointing_slot (#vcfg:_) 
-                (st:vstore vcfg) 
+let pointing_slot (#vcfg:_)
+                (st:vstore vcfg)
                 (s:inuse_slot_id st{Root <> stored_key st s /\ add_method_of st s = Spec.MAdd})
  : Tot (s':inuse_slot_id st{points_to st s' s}) = admit()
 
@@ -669,14 +670,14 @@ let lemma_ismap_madd_to_store (#vcfg:_) (st:ismap_vstore vcfg)
           (ensures (is_map (madd_to_store st s k v s' d)))
   = admit()
 
-let lemma_ismap_madd_to_store_split 
+let lemma_ismap_madd_to_store_split
   (#vcfg: verifier_config)
   (st:ismap_vstore vcfg)
   (s:empty_slot_id st)
   (k:key) (v:value_type_of k)
   (s':merkle_slot_id st)
   (d:bin_tree_dir {points_to_some_slot st s' d})
-  (d2:bin_tree_dir)  
+  (d2:bin_tree_dir)
   : Lemma (requires (not (store_contains_key st k)))
           (ensures (is_map (madd_to_store_split st s k v s' d d2)))
   = admit()
@@ -695,9 +696,9 @@ let lemma_empty_contains_nokey (#vcfg:_) (k:key):
 
 let lemma_madd_root_to_store_is_map
       (#vcfg:_)
-      (st:ismap_vstore vcfg{not (store_contains_key st Root)}) 
-      (s:empty_slot_id st) 
-      (v:value_type_of Root) 
+      (st:ismap_vstore vcfg{not (store_contains_key st Root)})
+      (s:empty_slot_id st)
+      (v:value_type_of Root)
   : Lemma (ensures (is_map (madd_to_store_root st s v))) = admit()
 
 let lemma_as_map_empty (vcfg:_)
@@ -720,13 +721,13 @@ let slot_of_key (#vcfg:_) (st:ismap_vstore vcfg) (k: key{let stk = as_map st in
 
 (*
 (* update the data value of a data key *)
-let update_data_value 
+let update_data_value
   (st:vstore)
   (s:data_slot_id st)
   (v:value{DVal? v})
   : Tot (st':vstore {Seq.length st = Seq.length st' /\
                      inuse_slot st' s /\
-                     stored_value st' s = v}) = 
+                     stored_value st' s = v}) =
   assert(not (desc_in_store st s Left));
   assert(not (desc_in_store st s Right));
   let Some (VStoreE k _ am _ _) = get_slot st s in
@@ -737,13 +738,13 @@ let update_data_value
 
   let aux1 (s0:slot_id st'):
     Lemma (ensures (inuse_slot st' s0 = inuse_slot st s0 /\
-                    (inuse_slot st' s0 ==> 
+                    (inuse_slot st' s0 ==>
                      stored_key st' s0 = stored_key st s0))) = ()
   in
 
   let aux (s0:slot_id st'):
     Lemma (ensures (store_inv_slot st' s0))
-          [SMTPat (store_inv_slot st' s0)] = 
+          [SMTPat (store_inv_slot st' s0)] =
     if s0 = s then ()
     else (
       assert(Seq.index st s0 = Seq.index st' s0);
@@ -757,7 +758,7 @@ let update_data_value
   st'
 
 
-let lemma_lookup_key_returns_k (st:vstore) (k:key) 
+let lemma_lookup_key_returns_k (st:vstore) (k:key)
   : Lemma (requires (store_contains_key st k))
           (ensures (VStoreE?.k (Some?.v (lookup_key st k)) = k))
   = lemma_filter_correct1 (has_key k) st 0
@@ -765,7 +766,7 @@ let lemma_lookup_key_returns_k (st:vstore) (k:key)
 let lemma_lookup_key_returns_None (st:vstore) (k:key)
   : Lemma (requires (lookup_key st k = None))
           (ensures (forall i. not (has_key k (Seq.index st i))))
-  = if Seq.length (filter (has_key k) st) = 0 
+  = if Seq.length (filter (has_key k) st) = 0
     then lemma_filter_all_not (has_key k) st
     else lemma_filter_correct1 (has_key k) st 0
 
@@ -784,8 +785,8 @@ let lemma_store_contains_key_inv (st:vstore) (k:key)
   : Lemma (requires (store_contains_key st k))
           (ensures (exists s. stored_key st s = k))
   = let s' = filter (has_key k) st in
-    if Seq.length s' > 0 
-    then 
+    if Seq.length s' > 0
+    then
       let i = filter_index_map (has_key k) st 0 in
       lemma_has_key st i k
 
@@ -798,16 +799,16 @@ let add_method_of_by_key (st:vstore) (k:key{store_contains_key st k})
   : add_method
   = VStoreE?.am (Some?.v (lookup_key st k))
 
-(* Two cases where it's safe to add an entry (e) to the store (st) at slot s: 
+(* Two cases where it's safe to add an entry (e) to the store (st) at slot s:
    * e.k is not in st and s is empty
    * e.k is already at s *)
 let compatible_entry (st:vstore) (s:st_index st) (e:vstore_entry)
-  = (not (store_contains st s) /\ not (store_contains_key st e.k)) \/ 
-    (store_contains st s /\ stored_key st s = e.k) 
+  = (not (store_contains st s) /\ not (store_contains_key st e.k)) \/
+    (store_contains st s /\ stored_key st s = e.k)
 
-let lemma_update_slot_compatible_entry_is_map 
-      (st:vstore{is_map st}) 
-      (s:st_index st) 
+let lemma_update_slot_compatible_entry_is_map
+      (st:vstore{is_map st})
+      (s:st_index st)
       (e:vstore_entry{compatible_entry st s e})
   : Lemma (is_map (update_slot st s e))
           [SMTPat (is_map (update_slot st s e))]
@@ -816,44 +817,44 @@ let lemma_update_slot_compatible_entry_is_map
             (s0':slot_id{store_contains st_upd s0' /\ s0' <> s0})
           : Lemma (stored_key st_upd s0 <> stored_key st_upd s0')
                   [SMTPat (Seq.index st_upd s0); SMTPat (Seq.index st_upd s0')]
-          = if s0 = s 
+          = if s0 = s
             then assert (stored_key st s0' <> e.k)
-            else if s0' = s 
+            else if s0' = s
             then assert (stored_key st s0 <> e.k) in
     assert (is_map st_upd)
 
 let lemma_add_to_store_is_map1
-      (st:vstore) 
-      (s:st_index st{not (store_contains st s)}) 
-      (k:key{not (store_contains_key st k)}) 
-      (v:value_type_of k) 
+      (st:vstore)
+      (s:st_index st{not (store_contains st s)})
+      (k:key{not (store_contains_key st k)})
+      (v:value_type_of k)
       (am:add_method)
   : Lemma (requires (is_map st))
           (ensures (is_map (add_to_store st s k v am)))
   = () // proved by lemma_update_compatible_entry_is_map
-  
+
 let lemma_add_to_store_is_map2
-      (st:vstore) 
-      (s:st_index st{not (store_contains st s)}) 
-      (k:key{store_contains_key st k}) 
-      (v:value_type_of k) 
+      (st:vstore)
+      (s:st_index st{not (store_contains st s)})
+      (k:key{store_contains_key st k})
+      (v:value_type_of k)
       (am:add_method)
   : Lemma (ensures (~ (is_map (add_to_store st s k v am))))
   = let st_upd = add_to_store st s k v am in
     assert (stored_key st_upd s = k);
     lemma_store_contains_key_inv st k;
-    Classical.exists_elim 
-      (exists (s':slot_id{store_contains st_upd s' /\ s' <> s}). 
-      stored_key st_upd s' = stored_key st_upd s) 
-      (Squash.get_proof (exists s. stored_key st s = k)) 
+    Classical.exists_elim
+      (exists (s':slot_id{store_contains st_upd s' /\ s' <> s}).
+      stored_key st_upd s' = stored_key st_upd s)
+      (Squash.get_proof (exists s. stored_key st s = k))
       (fun s' -> assert (stored_key st_upd s' = k));
     // we have shown two different slots with the same key, so the invariant is violated
     ()
- 
-let lemma_lookup_key_update_value 
-      (st:vstore) 
-      (s:slot_id{store_contains st s}) 
-      (v:value_type_of (stored_key st s)) 
+
+let lemma_lookup_key_update_value
+      (st:vstore)
+      (s:slot_id{store_contains st s})
+      (v:value_type_of (stored_key st s))
       (k:key)
   : Lemma (let res = lookup_key st k in
            let res' = lookup_key (update_value st s v) k in
@@ -862,7 +863,7 @@ let lemma_lookup_key_update_value
   = let stf = filter (has_key k) st in
     let Some (VStoreE ks _ am l r) = Seq.index st s in
     assert (Seq.length stf = Seq.length (filter (has_key k) (update_value st s v)));
-    if Seq.length stf > 0 
+    if Seq.length stf > 0
     then (
       if filter_index_map (has_key k) st 0 = s
       then lemma_filter_update_index_eq (has_key k) st s (Some (VStoreE ks v am l r))
@@ -870,8 +871,8 @@ let lemma_lookup_key_update_value
     )
 
 let lemma_update_value_preserves_keys
-      (st:vstore) 
-      (s:slot_id{store_contains st s}) 
+      (st:vstore)
+      (s:slot_id{store_contains st s})
       (v:value_type_of (stored_key st s))
       (k:key)
   : Lemma (store_contains_key st k = store_contains_key (update_value st s v) k)
@@ -879,16 +880,16 @@ let lemma_update_value_preserves_keys
 
 let lemma_update_value_preserves_key_with_MAdd
   (st:vstore)
-  (s:slot_id{store_contains st s}) 
+  (s:slot_id{store_contains st s})
   (v:value_type_of (stored_key st s))
   (k:key)
-  : Lemma (ensures store_contains_key_with_MAdd st k = 
+  : Lemma (ensures store_contains_key_with_MAdd st k =
                      store_contains_key_with_MAdd (update_value st s v) k)
   = lemma_lookup_key_update_value st s v k
 
 let lemma_add_different_key_to_store_preserves_keys_with_MAdd
   (st:vstore)
-  (s:st_index st{not (store_contains st s)}) 
+  (s:st_index st{not (store_contains st s)})
   (k:key)
   (v:value_type_of k)
   (k0:key)
@@ -901,14 +902,14 @@ let lemma_add_different_key_to_store_preserves_keys_with_MAdd
       assert (filter_index_map (has_key k0) st 0 <> s);
       lemma_filter_update_index_neq (has_key k0) st s (Some (VStoreE k v Spec.MAdd false false)) 0
     )
-    
+
 let lemma_add_to_store_BAdd_preserves_key_with_MAdd
   (st:vstore)
-  (s:st_index st{not (store_contains st s)}) 
+  (s:st_index st{not (store_contains st s)})
   (k:key{not (store_contains_key st k)})
   (v:value_type_of k)
   (k0:key)
-  : Lemma (ensures store_contains_key_with_MAdd st k0 = 
+  : Lemma (ensures store_contains_key_with_MAdd st k0 =
                      store_contains_key_with_MAdd (add_to_store st s k v Spec.BAdd) k0)
   = let stf = filter (has_key k0) st in
     if Seq.length stf = 0
@@ -927,11 +928,11 @@ let lemma_add_to_store_BAdd_preserves_key_with_MAdd
       assert (k <> k0);
       assert (filter_index_map (has_key k0) st 0 <> s);
       lemma_filter_update_index_neq (has_key k0) st s (Some (VStoreE k v Spec.BAdd false false)) 0
-    )    
+    )
 
 let lemma_add_to_store_MAdd_adds_key_with_MAdd
   (st:vstore)
-  (s:st_index st{not (store_contains st s)}) 
+  (s:st_index st{not (store_contains st s)})
   (k:key{not (store_contains_key st k)})
   (v:value_type_of k)
   : Lemma (ensures store_contains_key_with_MAdd (add_to_store st s k v Spec.MAdd) k)
@@ -942,9 +943,9 @@ let lemma_add_to_store_MAdd_adds_key_with_MAdd
     assert (forall j. j <> s ==> not (has_key k (Seq.index st_upd j)));
     lemma_filter_unique (has_key k) st_upd s
 
-let lemma_lookup_key_update_in_store 
-      (st:vstore) 
-      (s:slot_id{store_contains st s}) 
+let lemma_lookup_key_update_in_store
+      (st:vstore)
+      (s:slot_id{store_contains st s})
       (d:bin_tree_dir)
       (b:bool)
       (k:key)
@@ -958,7 +959,7 @@ let lemma_lookup_key_update_in_store
                   | Left -> Some (VStoreE ks v am b r)
                   | Right -> Some (VStoreE ks v am l b) in
     assert (Seq.length stf = Seq.length (filter (has_key k) (update_in_store st s d b)));
-    if Seq.length stf > 0 
+    if Seq.length stf > 0
     then (
       (** TODO: For some reason this started failing with the updated vevictb/vevictbm *)
       (*
@@ -971,7 +972,7 @@ let lemma_lookup_key_update_in_store
 
 let lemma_update_in_store_preserves_keys
   (st:vstore)
-  (s:st_index st{store_contains st s}) 
+  (s:st_index st{store_contains st s})
   (d:bin_tree_dir)
   (b:bool)
   (k:key)
@@ -980,17 +981,17 @@ let lemma_update_in_store_preserves_keys
 
 let lemma_update_in_store_preserves_key_with_MAdd
   (st:vstore)
-  (s:st_index st{store_contains st s}) 
+  (s:st_index st{store_contains st s})
   (d:bin_tree_dir)
   (b:bool)
   (k:key)
-  : Lemma (ensures store_contains_key_with_MAdd st k = 
+  : Lemma (ensures store_contains_key_with_MAdd st k =
                      store_contains_key_with_MAdd (update_in_store st s d b) k)
   = lemma_lookup_key_update_in_store st s d b k
 
 let lemma_evict_from_store_evicts_key
   (st:vstore)
-  (s:st_index st{store_contains st s}) 
+  (s:st_index st{store_contains st s})
   : Lemma (requires is_map st)
           (ensures not (store_contains_key (evict_from_store st s) (stored_key st s)))
   = let k = stored_key st s in
@@ -1000,8 +1001,8 @@ let lemma_evict_from_store_evicts_key
     assert (Seq.length res = 0)
 
 let lemma_lookup_key_evict_from_store
-      (st:vstore) 
-      (s:slot_id{store_contains st s}) 
+      (st:vstore)
+      (s:slot_id{store_contains st s})
       (k:key{k <> stored_key st s})
   : Lemma (lookup_key st k = lookup_key (evict_from_store st s) k)
   = let stf = filter (has_key k) st in
@@ -1013,7 +1014,7 @@ let lemma_lookup_key_evict_from_store
 
 let lemma_evict_from_store_preserves_key_with_MAdd
   (st:vstore)
-  (s:st_index st{store_contains st s}) 
+  (s:st_index st{store_contains st s})
   (k:key)
   : Lemma (requires (k <> stored_key st s))
           (ensures (store_contains_key_with_MAdd st k = store_contains_key_with_MAdd (evict_from_store st s) k))
@@ -1027,45 +1028,45 @@ let lemma_get_slot_lookup_key (st:vstore{is_map st}) (s:slot_id) (k:key)
 
 let lemma_evict_from_store_BAdd_preserves_key_with_MAdd
   (st:vstore{is_map st})
-  (s:slot_id{store_contains st s}) 
+  (s:slot_id{store_contains st s})
   (k:key)
   : Lemma (requires (add_method_of st s = Spec.BAdd))
-          (ensures (store_contains_key_with_MAdd st k = 
+          (ensures (store_contains_key_with_MAdd st k =
                       store_contains_key_with_MAdd (evict_from_store st s) k))
   = if k = stored_key st s
     then lemma_get_slot_lookup_key st s k
     else lemma_lookup_key_evict_from_store st s k
 
-let lemma_slot_key_equiv_update_value 
-      (st:vstore) 
-      (s:slot_id) 
-      (s':slot_id{store_contains st s'}) 
-      (k:key) 
+let lemma_slot_key_equiv_update_value
+      (st:vstore)
+      (s:slot_id)
+      (s':slot_id{store_contains st s'})
+      (k:key)
       (v:value_type_of (stored_key st s'))
   : Lemma (requires (slot_key_equiv st s k /\ s <> s'))
           (ensures (slot_key_equiv (update_value st s' v) s k))
   = ()
 
-let rec as_map_aux (l:vstore) 
+let rec as_map_aux (l:vstore)
   : Tot Spec.vstore (decreases (Seq.length l)) =
   let n = Seq.length l in
   if n = 0 then Spec.empty_store
-  else 
+  else
     let l' = prefix l (n - 1) in
     let f' = as_map_aux l' in
     match Seq.index l (n - 1) with
     | None -> f'
-    | Some (VStoreE k v a _ _) -> 
+    | Some (VStoreE k v a _ _) ->
       Spec.add_to_store f' k v a
 
 let as_map (st:vstore{is_map st}) : Spec.vstore =
   as_map_aux st
 
-let rec lemma_as_map_empty (n:nat) 
+let rec lemma_as_map_empty (n:nat)
   : Lemma (ensures (let st = empty_store n in
                      forall (k:key). as_map st k = None))
           (decreases n)
-  = if n <> 0 
+  = if n <> 0
     then (
       lemma_prefix_create n (None #vstore_entry) (n-1);
       lemma_as_map_empty (n-1)
@@ -1077,46 +1078,46 @@ let lemma_is_map_prefix (l:vstore) (i:seq_index l)
           [SMTPat (is_map (prefix l i))]
   = ()
 
-let rec lemma_as_map_slot_key_equiv_aux 
-      (l:vstore) 
-      (s:slot_id) 
-      (k:key) 
-      (v:value_type_of k) 
+let rec lemma_as_map_slot_key_equiv_aux
+      (l:vstore)
+      (s:slot_id)
+      (k:key)
+      (v:value_type_of k)
       (am:add_method)
       (lb rb:bool)
-  : Lemma (requires (s < Seq.length l /\ 
+  : Lemma (requires (s < Seq.length l /\
                      Seq.index l s = Some (VStoreE k v am lb rb) /\
-                     is_map l)) 
+                     is_map l))
           (ensures (Spec.store_contains (as_map_aux l) k /\
                     Spec.stored_value (as_map_aux l) k = v /\
                     Spec.add_method_of (as_map_aux l) k = am))
           (decreases (Seq.length l))
   = let n = Seq.length l in
-    if n <> 0 
+    if n <> 0
     then
       let l' = prefix l (n - 1) in
       match Seq.index l (n - 1) with
       | None -> lemma_as_map_slot_key_equiv_aux l' s k v am lb rb
-      | Some (VStoreE k2 v2 am2 _ _) -> 
-          if s < n - 1 
+      | Some (VStoreE k2 v2 am2 _ _) ->
+          if s < n - 1
           then lemma_as_map_slot_key_equiv_aux l' s k v am lb rb
 
 let lemma_as_map_slot_key_equiv (st:vstore{is_map st}) (s:slot_id) (k:key)
-  : Lemma (requires (slot_key_equiv st s k)) 
+  : Lemma (requires (slot_key_equiv st s k))
           (ensures (Spec.store_contains (as_map st) k /\
                     stored_value st s = Spec.stored_value (as_map st) k /\
-                    add_method_of st s = Spec.add_method_of (as_map st) k)) 
-  = let Some (VStoreE k v a l r) = get_slot st s in 
+                    add_method_of st s = Spec.add_method_of (as_map st) k))
+  = let Some (VStoreE k v a l r) = get_slot st s in
     lemma_as_map_slot_key_equiv_aux st s k v a l r
 
-let rec lemma_as_map_aux_does_not_contain_key 
-      (l:vstore) 
-      (k:key) 
-  : Lemma (requires (forall i. not (has_key k (Seq.index l i)))) 
+let rec lemma_as_map_aux_does_not_contain_key
+      (l:vstore)
+      (k:key)
+  : Lemma (requires (forall i. not (has_key k (Seq.index l i))))
           (ensures (not (Spec.store_contains (as_map_aux l) k)))
           (decreases (Seq.length l))
   = let n = Seq.length l in
-    if n <> 0 
+    if n <> 0
     then
       let l' = prefix l (n - 1) in
       lemma_as_map_aux_does_not_contain_key l' k
@@ -1127,9 +1128,9 @@ let lemma_store_rel_contains_key (st:vstore) (st':Spec.vstore) (k:key)
   = if store_contains_key st k
     then (
       lemma_store_contains_key_inv st k;
-      Classical.exists_elim 
-        (Spec.store_contains (as_map st) k) 
-        (Squash.get_proof (exists s. slot_key_equiv st s k)) 
+      Classical.exists_elim
+        (Spec.store_contains (as_map st) k)
+        (Squash.get_proof (exists s. slot_key_equiv st s k))
         (fun s -> lemma_as_map_slot_key_equiv st s k)
     )
     else (
@@ -1141,20 +1142,20 @@ let lemma_store_rel_stored_value (st:vstore) (st':Spec.vstore) (k:key)
   : Lemma (requires (store_rel st st' /\ store_contains_key st k))
           (ensures (stored_value_by_key st k = Spec.stored_value st' k))
   = lemma_store_contains_key_inv st k;
-    Classical.exists_elim 
-      (stored_value_by_key st k = Spec.stored_value (as_map st) k) 
-      (Squash.get_proof (exists s. slot_key_equiv st s k)) 
-      (fun s -> lemma_get_slot_lookup_key st s k; 
+    Classical.exists_elim
+      (stored_value_by_key st k = Spec.stored_value (as_map st) k)
+      (Squash.get_proof (exists s. slot_key_equiv st s k))
+      (fun s -> lemma_get_slot_lookup_key st s k;
              lemma_as_map_slot_key_equiv st s k)
-   
+
 let lemma_store_rel_add_method_of (st:vstore) (st':Spec.vstore) (k:key)
   : Lemma (requires (store_rel st st' /\ store_contains_key st k))
           (ensures (add_method_of_by_key st k = Spec.add_method_of st' k))
   = lemma_store_contains_key_inv st k;
-    Classical.exists_elim 
-      (add_method_of_by_key st k = Spec.add_method_of (as_map st) k) 
-      (Squash.get_proof (exists s. slot_key_equiv st s k)) 
-      (fun s -> lemma_get_slot_lookup_key st s k; 
+    Classical.exists_elim
+      (add_method_of_by_key st k = Spec.add_method_of (as_map st) k)
+      (Squash.get_proof (exists s. slot_key_equiv st s k))
+      (fun s -> lemma_get_slot_lookup_key st s k;
              lemma_as_map_slot_key_equiv st s k)
 
 let compatible_entry_prefix (st:vstore) (s:st_index st) (e:vstore_entry) (i:st_index st)
@@ -1168,23 +1169,23 @@ let compatible_entry_prefix (st:vstore) (s:st_index st) (e:vstore_entry) (i:st_i
     )
 
 #push-options "--fuel 1,1 --ifuel 2,2"
-let rec lemma_as_map_update (st:vstore{is_map st}) 
+let rec lemma_as_map_update (st:vstore{is_map st})
                             (s:st_index st)
                             (e:vstore_entry{compatible_entry st s e})
   : Lemma (ensures (let m = as_map st in
                     let m' = as_map (update_slot st s e) in
                     m' e.k = Some (Spec.VStore e.v e.am) /\
-                    (forall k. k <> e.k ==> m' k = m k))) 
+                    (forall k. k <> e.k ==> m' k = m k)))
           (decreases (Seq.length st))
   = let n = Seq.length st in
-    if n <> 0 
+    if n <> 0
     then
       let st_upd = update_slot st s e in
       let st_p = prefix st (n - 1) in
       let st_upd_p = prefix st_upd (n - 1) in
       if s < n - 1
-      then ( 
-        let st_p_upd = update_slot st_p s e in      
+      then (
+        let st_p_upd = update_slot st_p s e in
         lemma_as_map_update st_p s e;
         assert (Seq.equal st_p_upd st_upd_p)
       )
@@ -1204,7 +1205,7 @@ let lemma_store_rel_update_in_store (st:vstore) (st':Spec.vstore) (s:slot_id) (d
           (ensures (store_rel (update_in_store st s d b) st'))
   = let Some (VStoreE k v am l r) = get_slot st s in
     assert (slot_key_equiv st s k); // assert needed to trigger pattern
-    let e = match d with 
+    let e = match d with
             | Left -> VStoreE k v am b r
             | Right -> VStoreE k v am l b in
     lemma_as_map_update st s e
@@ -1218,16 +1219,16 @@ let rec lemma_as_map_evict (st:vstore{is_map st}) (s:st_index st) (k:key)
   : Lemma (requires (slot_key_equiv st s k))
           (ensures (let m = as_map st in
                     let m' = as_map (evict_from_store st s) in
-                    m' k = None /\ (forall k'. k' <> k ==> m' k' = m k'))) 
+                    m' k = None /\ (forall k'. k' <> k ==> m' k' = m k')))
           (decreases (Seq.length st))
   = let n = Seq.length st in
-    if n <> 0 
+    if n <> 0
     then
       let stupd = evict_from_store st s in
       let stp = prefix st (n - 1) in
       let stupdp = prefix stupd (n - 1) in
       if s < n - 1
-      then ( 
+      then (
         lemma_as_map_evict stp s k;
         assert (Seq.equal stupdp (evict_from_store stp s))
       )
