intermediate/Veritas.Intermediate.Thread.fst
@@ -1,21 +1,21 @@
 module Veritas.Intermediate.Thread
 
 let lemma_init_store_ismap (vcfg:verifier_config) (tid:thread_id)
-  : Lemma (ensures (is_map (init_store vcfg tid))) = 
+  : Lemma (ensures (is_map (init_store vcfg tid))) =
   let st = empty_store vcfg in
-  lemma_empty_store_is_map #vcfg;  
+  lemma_empty_store_is_map #vcfg;
   lemma_empty_contains_nokey #vcfg Root;
   if tid = 0 then
-    lemma_madd_root_to_store_is_map st 0 (init_value Root)    
+    lemma_madd_root_to_store_is_map st 0 (init_value Root)
   else ()
-    
+
 let lemma_init_store_slot_points_to_is_merkle_points_to (vcfg:verifier_config) (tid:thread_id)
-  : Lemma (ensures (slot_points_to_is_merkle_points_to (init_store vcfg tid))) = 
+  : Lemma (ensures (slot_points_to_is_merkle_points_to (init_store vcfg tid))) =
   let st = init_store vcfg tid in
   let aux (s1 s2: slot_id vcfg) (d: bin_tree_dir):
-    Lemma (ensures (not (points_to_dir st s1 d s2))) 
-          [SMTPat (slot_points_to_is_merkle_points_to_local st s1 s2 d)] = 
-    if tid = 0 then   
+    Lemma (ensures (not (points_to_dir st s1 d s2)))
+          [SMTPat (slot_points_to_is_merkle_points_to_local st s1 s2 d)] =
+    if tid = 0 then
       ()
     else ()
   in
@@ -24,7 +24,7 @@ let lemma_init_store_slot_points_to_is_merkle_points_to (vcfg:verifier_config) (
 let rec verifiable_implies_prefix_verifiable_aux
   (#vcfg:_) (tl:verifiable_log vcfg) (i:nat{i <= length tl}):
   Lemma (ensures (verifiable (prefix tl i)))
-        (decreases (length tl)) = 
+        (decreases (length tl)) =
   let n = length tl in
   if i = n then ()
   else
@@ -32,9 +32,9 @@ let rec verifiable_implies_prefix_verifiable_aux
 
 let verifiable_implies_prefix_verifiable = verifiable_implies_prefix_verifiable_aux
 
-let rec blum_add_seq_aux (#vcfg:_) (tl: verifiable_log vcfg): 
+let rec blum_add_seq_aux (#vcfg:_) (tl: verifiable_log vcfg):
   Tot (S.seq ms_hashfn_dom)
-  (decreases (length tl)) = 
+  (decreases (length tl)) =
   let n = length tl in
   if n = 0 then S.empty #ms_hashfn_dom
   else
@@ -44,16 +44,16 @@ let rec blum_add_seq_aux (#vcfg:_) (tl: verifiable_log vcfg):
     if is_blum_add e then SA.append1 s' (blum_add_elem e)
     else s'
 
-let blum_add_seq (#vcfg:_) (tl: verifiable_log vcfg): S.seq ms_hashfn_dom = 
+let blum_add_seq (#vcfg:_) (tl: verifiable_log vcfg): S.seq ms_hashfn_dom =
   blum_add_seq_aux tl
 
 let rec add_seq_map_aux (#vcfg:_) (tl: verifiable_log vcfg) (i: seq_index tl{is_blum_add (index tl i)}):
   Tot (j: SA.seq_index (blum_add_seq tl){S.index (blum_add_seq tl) j =
                                      blum_add_elem (index tl i)})
-  (decreases (length tl)) = 
+  (decreases (length tl)) =
   let n = length tl in
   if n = 0 then 0
-  else 
+  else
     let tl' = prefix tl (n - 1) in
     let s' = blum_add_seq tl' in
     if i = n - 1 then
@@ -68,8 +68,8 @@ let add_seq_map (#vcfg:_) (tl: verifiable_log vcfg) (i: seq_index tl{is_blum_add
 let rec add_seq_inv_map_aux (#vcfg:_) (tl: verifiable_log vcfg) (j: SA.seq_index (blum_add_seq tl)):
   Tot (i: seq_index tl {is_blum_add (index tl i) /\
               blum_add_elem (index tl i) = S.index (blum_add_seq tl) j /\
-              add_seq_map tl i = j}) 
-  (decreases (length tl)) = 
+              add_seq_map tl i = j})
+  (decreases (length tl)) =
   let n = length tl in
   if n = 0 then 0
   else
@@ -77,7 +77,7 @@ let rec add_seq_inv_map_aux (#vcfg:_) (tl: verifiable_log vcfg) (j: SA.seq_index
     let s' = blum_add_seq_aux tl' in
     let e = index tl (n - 1) in
     let s = blum_add_seq tl in
-    if j = S.length s' then 
+    if j = S.length s' then
       n - 1
     else
       add_seq_inv_map_aux tl' j
@@ -89,7 +89,7 @@ let add_seq_inv_map (#vcfg:_) (tl: verifiable_log vcfg) (j: SA.seq_index (blum_a
 
 let rec lemma_add_seq_inv_aux (#vcfg:_) (tl: verifiable_log vcfg) (i: seq_index tl{is_blum_add (index tl i)}):
   Lemma (ensures (add_seq_inv_map tl (add_seq_map tl i) = i))
-        (decreases (length tl)) = 
+        (decreases (length tl)) =
   let n = length tl in
   assert (n > 0);
   let tl' = prefix tl (n - 1) in
@@ -99,7 +99,7 @@ let rec lemma_add_seq_inv_aux (#vcfg:_) (tl: verifiable_log vcfg) (i: seq_index 
 
   if i = n - 1 then ()
   else
-    lemma_add_seq_inv_aux tl' i 
+    lemma_add_seq_inv_aux tl' i
 
 let lemma_add_seq_inv (#vcfg:_) (tl: verifiable_log vcfg) (i: seq_index tl{is_blum_add (index tl i)}):
   Lemma (ensures (add_seq_inv_map tl (add_seq_map tl i) = i)) = lemma_add_seq_inv_aux tl i
@@ -113,11 +113,11 @@ let hadd_at #vcfg (tl: verifiable_log vcfg) (i:nat{i <= length tl}): ms_hash_val
 
 let lemma_state_transition #vcfg (tl: verifiable_log vcfg) (i: seq_index tl):
   Lemma (state_at tl (i + 1) ==
-         verify_step (state_at tl i) (index tl i)) = 
+         verify_step (state_at tl i) (index tl i)) =
   ()
 
 let lemma_hadd_unchanged #vcfg (tl: verifiable_log _) (i: seq_index tl{not (is_blum_add (index tl i))}):
-  Lemma (hadd_at tl i == hadd_at tl (i + 1)) = 
+  Lemma (hadd_at tl i == hadd_at tl (i + 1)) =
   lemma_state_transition #vcfg tl i;
   ()
 
@@ -133,16 +133,16 @@ let rec lemma_hadd_correct_aux #vcfg (tl: verifiable_log vcfg):
     let e = index tl (n - 1) in
     let h' = hadd tl' in
     lemma_hadd_correct_aux tl';
-    if is_blum_add e then lemma_hashfn_app s' (blum_add_elem e)      
-    else lemma_hadd_unchanged tl (n - 1)      
+    if is_blum_add e then lemma_hashfn_app s' (blum_add_elem e)
+    else lemma_hadd_unchanged tl (n - 1)
   )
 
 let lemma_hadd_correct (#vcfg:_) (tl: verifiable_log vcfg):
   Lemma (ensures (hadd tl = ms_hashfn (blum_add_seq tl))) = lemma_hadd_correct_aux tl
 
-let rec blum_evict_seq_aux #vcfg (tl: verifiable_log vcfg): 
+let rec blum_evict_seq_aux #vcfg (tl: verifiable_log vcfg):
   Tot (S.seq ms_hashfn_dom)
-  (decreases (length tl)) = 
+  (decreases (length tl)) =
   let n = length tl in
   if n = 0 then S.empty #ms_hashfn_dom
   else (
@@ -173,15 +173,15 @@ let rec lemma_thread_id_state #vcfg (tl: verifiable_log vcfg):
 module Spec = Veritas.Verifier
 
 let lemma_hevict_change #vcfg (tl: verifiable_log vcfg) (i: seq_index tl{is_evict_to_blum (index tl i)}):
-  Lemma (hevict_at tl (i + 1) = ms_hashfn_upd (blum_evict_elem tl i) (hevict_at tl i)) = 
-  lemma_state_transition tl i;  
+  Lemma (hevict_at tl (i + 1) = ms_hashfn_upd (blum_evict_elem tl i) (hevict_at tl i)) =
+  lemma_state_transition tl i;
   lemma_thread_id_state (prefix tl i)
 
 let rec lemma_hevict_correct_aux #vcfg (tl: verifiable_log vcfg):
   Lemma (ensures (hevict tl = ms_hashfn (blum_evict_seq tl)))
-        (decreases (length tl)) = 
+        (decreases (length tl)) =
   let n = length tl in
-  if n = 0 then 
+  if n = 0 then
     lemma_hashfn_empty()
   else (
     let tl' = prefix tl (n - 1) in
@@ -190,22 +190,22 @@ let rec lemma_hevict_correct_aux #vcfg (tl: verifiable_log vcfg):
     let e = index tl (n - 1) in
     let h' = hevict tl' in
     let h = hevict tl in
-    lemma_hevict_correct_aux tl';  
-    if is_evict_to_blum e then (    
+    lemma_hevict_correct_aux tl';
+    if is_evict_to_blum e then (
       lemma_hashfn_app s' (blum_evict_elem tl (n - 1));
       lemma_hevict_change tl (n - 1)
     )
     else
-      lemma_hevict_unchanged tl (n - 1)   
+      lemma_hevict_unchanged tl (n - 1)
   )
 
 let lemma_hevict_correct (#vcfg:_) (tl: verifiable_log vcfg):
   Lemma (hevict tl = ms_hashfn (blum_evict_seq tl)) = lemma_hevict_correct_aux tl
 
 let rec evict_seq_map_aux (#vcfg:_) (tl: verifiable_log vcfg) (i: seq_index tl{is_evict_to_blum (index tl i)}):
-  Tot (j: SA.seq_index (blum_evict_seq tl) {S.index (blum_evict_seq tl) j = 
-                                        blum_evict_elem tl i}) 
-  (decreases (length tl)) = 
+  Tot (j: SA.seq_index (blum_evict_seq tl) {S.index (blum_evict_seq tl) j =
+                                        blum_evict_elem tl i})
+  (decreases (length tl)) =
   let n = length tl in
   let tl' = prefix tl (n - 1) in
   let s' = blum_evict_seq tl' in
@@ -215,14 +215,14 @@ let rec evict_seq_map_aux (#vcfg:_) (tl: verifiable_log vcfg) (i: seq_index tl{i
     evict_seq_map_aux tl' i
 
 let evict_seq_map (#vcfg:_) (tl: verifiable_log vcfg) (i: seq_index tl{is_evict_to_blum (index tl i)}):
-  (j: SA.seq_index (blum_evict_seq tl) {S.index (blum_evict_seq tl) j = 
+  (j: SA.seq_index (blum_evict_seq tl) {S.index (blum_evict_seq tl) j =
                                         blum_evict_elem tl i}) = evict_seq_map_aux tl i
 
 let rec evict_seq_inv_map_aux (#vcfg:_) (tl: verifiable_log vcfg) (j: SA.seq_index (blum_evict_seq tl)):
   Tot (i: seq_index tl{is_evict_to_blum (index tl i) /\
              blum_evict_elem tl i = S.index (blum_evict_seq tl) j /\
              evict_seq_map tl i = j})
-  (decreases (length tl)) = 
+  (decreases (length tl)) =
   let n = length tl in
   let tl' = prefix tl (n - 1) in
   let s' = blum_evict_seq tl' in
@@ -248,14 +248,14 @@ let rec lemma_evict_seq_inv_aux (#vcfg:_) (tl: verifiable_log vcfg) (i: seq_inde
 let lemma_evict_seq_inv (#vcfg:_) (tl: verifiable_log vcfg) (i: seq_index tl{is_evict_to_blum (index tl i)}):
   Lemma (ensures (evict_seq_inv_map tl (evict_seq_map tl i) = i)) = lemma_evict_seq_inv_aux tl i
 
-let lemma_blum_evict_elem_prefix (#vcfg:_) (tl: verifiable_log vcfg) (i: nat{i <= length tl}) 
+let lemma_blum_evict_elem_prefix (#vcfg:_) (tl: verifiable_log vcfg) (i: nat{i <= length tl})
   (j: nat{j < i && is_evict_to_blum (index tl j)}):
   Lemma (blum_evict_elem tl j = blum_evict_elem (prefix tl i) j) = ()
 
 #push-options "--max_fuel 1 --max_ifuel 0"
 
 let lemma_add_clock (#vcfg:_) (tl: verifiable_log vcfg) (i: seq_index tl{is_blum_add (index tl i)}):
-  Lemma (timestamp_of (blum_add_elem (index tl i)) `ts_lt`  clock tl i) = 
+  Lemma (timestamp_of (blum_add_elem (index tl i)) `ts_lt`  clock tl i) =
   let e = index tl i in
   lemma_state_transition tl i;
   let si = state_at tl i in
@@ -268,7 +268,7 @@ let lemma_add_clock (#vcfg:_) (tl: verifiable_log vcfg) (i: seq_index tl{is_blum
 #pop-options
 
 let lemma_evict_clock (#vcfg:_) (tl: verifiable_log vcfg) (i: seq_index tl{is_evict_to_blum (index tl i)}):
-  Lemma (timestamp_of (blum_evict_elem tl i) = clock tl i)  = 
+  Lemma (timestamp_of (blum_evict_elem tl i) = clock tl i)  =
   let e = index tl i in
   lemma_state_transition tl i;
   let si = state_at tl i in
@@ -281,9 +281,9 @@ let lemma_evict_clock (#vcfg:_) (tl: verifiable_log vcfg) (i: seq_index tl{is_ev
 module MH = Veritas.MultiSetHash
 
 let rec lemma_evict_elem_tid_aux #vcfg (tl:verifiable_log vcfg) (i: SA.seq_index (blum_evict_seq tl)):
-  Lemma (ensures (MH.thread_id_of (S.index (blum_evict_seq tl) i) = (thread_id_of tl))) 
+  Lemma (ensures (MH.thread_id_of (S.index (blum_evict_seq tl) i) = (thread_id_of tl)))
         (decreases (length tl))
-        [SMTPat (is_of_thread_id (thread_id_of tl) (S.index (blum_evict_seq tl) i))] = 
+        [SMTPat (is_of_thread_id (thread_id_of tl) (S.index (blum_evict_seq tl) i))] =
   let es = blum_evict_seq tl in
   let tid = thread_id_of tl in
   let n = length tl in
@@ -296,21 +296,21 @@ let rec lemma_evict_elem_tid_aux #vcfg (tl:verifiable_log vcfg) (i: SA.seq_index
       if i = S.length es - 1 then
         ()
       else
-        lemma_evict_elem_tid_aux tl' i    
+        lemma_evict_elem_tid_aux tl' i
     else
-      lemma_evict_elem_tid_aux tl' i    
-  
+      lemma_evict_elem_tid_aux tl' i
+
 let lemma_evict_elem_tid (#vcfg:_) (tl:verifiable_log vcfg):
   Lemma (all (is_of_thread_id (thread_id_of tl)) (blum_evict_seq tl)) = ()
 
-let clock_pre #vcfg (tl:verifiable_log vcfg) (i:seq_index tl): timestamp = 
+let clock_pre #vcfg (tl:verifiable_log vcfg) (i:seq_index tl): timestamp =
   Valid?.clock (state_at tl i)
 
 let lemma_evict_clock_strictly_increasing #vcfg (tl: verifiable_log vcfg) (i: seq_index tl {is_evict_to_blum (index tl i)}):
   Lemma (ts_lt (clock_pre tl i) (clock tl i)) = ()
 
 let lemma_evict_timestamp_is_clock #vcfg (tl: verifiable_log vcfg) (i: seq_index tl{is_evict_to_blum (index tl i)}):
-  Lemma (timestamp_of (blum_evict_elem tl i) = clock tl i) = 
+  Lemma (timestamp_of (blum_evict_elem tl i) = clock tl i) =
   ()
 
 let final_clock #vcfg (tl:verifiable_log vcfg): timestamp =
@@ -330,20 +330,26 @@ let rec lemma_clock_monotonic_aux #vcfg (tl:verifiable_log vcfg) (i:seq_index tl
     lemma_clock_monotonic_aux tl' i
 #pop-options
 
+#push-options "--max_fuel 1 --max_ifuel 0"
 let lemma_clock_monotonic #vcfg (tl: verifiable_log vcfg) (i:seq_index tl) (j:seq_index tl{j >= i}):
   Lemma (clock tl i `ts_leq` clock tl j) =
   let tlj = prefix tl (j + 1) in
   lemma_clock_monotonic_aux tlj i
+  // assert(clock tlj i `ts_leq` clock tlj j);
+  // assert(clock tlj i = clock tl i);
+  // assert(clock tlj j = clock tl j);
+  //()
+#pop-options
 
 let lemma_final_clock_monotonic #vcfg (tl: verifiable_log vcfg) (i:seq_index tl):
-  Lemma (ts_leq (final_clock (prefix tl i)) (final_clock tl)) = 
+  Lemma (ts_leq (final_clock (prefix tl i)) (final_clock tl)) =
   if i = 0 then ()
   else
     lemma_clock_monotonic tl (i - 1) (length tl - 1)
 
 let rec lemma_evict_clock_leq_final_clock #vcfg (tl:verifiable_log vcfg) (i: SA.seq_index (blum_evict_seq tl)):
   Lemma (ensures (ts_leq (timestamp_of (S.index (blum_evict_seq tl) i)) (final_clock tl)))
-        (decreases (length tl)) = 
+        (decreases (length tl)) =
   let n = length tl in
   let es = blum_evict_seq tl in
   let be = S.index es i in
@@ -354,20 +360,20 @@ let rec lemma_evict_clock_leq_final_clock #vcfg (tl:verifiable_log vcfg) (i: SA.
     let tl' = prefix tl (n - 1) in
     let es' = blum_evict_seq tl' in
     let c' = final_clock tl' in
-    
+
     lemma_final_clock_monotonic tl (n - 1);
     assert(ts_leq c' c);
-    
-    if i < S.length es' then 
-      lemma_evict_clock_leq_final_clock tl' i    
-    else 
+
+    if i < S.length es' then
+      lemma_evict_clock_leq_final_clock tl' i
+    else
       lemma_evict_timestamp_is_clock tl (n - 1)
   )
 
 let rec lemma_evict_seq_clock_strictly_monotonic #vcfg (tl: verifiable_log vcfg) (i1 i2: SA.seq_index (blum_evict_seq tl)):
   Lemma (requires (i1 < i2))
-        (ensures (ts_lt (timestamp_of (S.index (blum_evict_seq tl) i1)) 
-                        (timestamp_of (S.index (blum_evict_seq tl) i2)))) 
+        (ensures (ts_lt (timestamp_of (S.index (blum_evict_seq tl) i1))
+                        (timestamp_of (S.index (blum_evict_seq tl) i2))))
         (decreases (length tl)) =
   let n = length tl in
   let es = blum_evict_seq tl in
@@ -381,11 +387,11 @@ let rec lemma_evict_seq_clock_strictly_monotonic #vcfg (tl: verifiable_log vcfg)
       let e = index tl (n - 1) in
       //assert(is_evict_to_blum e);
       //assert(timestamp_of (S.index (blum_evict_seq tl) i2) = timestamp_of (blum_evict_elem tl (n - 1)));
-             
+
       lemma_evict_timestamp_is_clock tl (n - 1);
       //assert(timestamp_of (blum_evict_elem tl (n - 1)) =  clock tl (n - 1));
-             
-      lemma_evict_clock_strictly_increasing tl (n - 1);             
+
+      lemma_evict_clock_strictly_increasing tl (n - 1);
       //assert(ts_lt (clock_pre tl (n - 1)) (clock tl (n - 1)));
       //assert(i1 < S.length es');
       //assert(S.index es i1 = S.index es' i1);
@@ -395,10 +401,9 @@ let rec lemma_evict_seq_clock_strictly_monotonic #vcfg (tl: verifiable_log vcfg)
   )
 
 let lemma_evict_elem_unique (#vcfg:_) (tl: verifiable_log vcfg) (i1 i2: SA.seq_index (blum_evict_seq tl)):
-  Lemma (i1 <> i2 ==> S.index (blum_evict_seq tl) i1 <> S.index (blum_evict_seq tl) i2) = 
+  Lemma (i1 <> i2 ==> S.index (blum_evict_seq tl) i1 <> S.index (blum_evict_seq tl) i2) =
   if i1 = i2 then ()
   else if i1 < i2 then
     lemma_evict_seq_clock_strictly_monotonic tl i1 i2
-  else 
+  else
     lemma_evict_seq_clock_strictly_monotonic tl i2 i1
- 
